---
title: "Lagrange's mean value theorem"
---

$\frac{f(b) - f(a)}{b - a}=f'(c)$

- Two real numbers $a < b$
- Function $f(x)$.
    - Continuous on closed interval $[a, b$]
    - Differentiable on open interval [$ (a, b)
- In this case, there exists a point $c$ on the open interval $(a, b)$ and the following holds
- $\frac{f(b) - f(a)}{b - a}=f'(c)$
- This is called Lagrange's mean value theorem for derivatives.
- As a separate expression, there exists a [$ 0 < \theta < 1
- $f(a + h) = f(a) + h f'(a + \theta h)$
    - Only the following rewrite is done $b = a + h, c = a + \theta h$.

By Lagrange's mean value theorem $\log(1 + x) = \frac{x}{1 + \theta x}$
- because
- $a = 1, h = x$ as
- $\log(1+x) = \log(1) + x \log'(1 + \theta x)$
- $\log'(x) = 1/x, \log(1) = 0$, so
- $\log(1 + x) = \frac{x}{1 + \theta x}$
- Since log(x) is not differentiable at x=0, the absolute value of x must be less than 1

---
This page is auto-translated from [/nishio/ラグランジュの平均値の定理](https://scrapbox.io/nishio/ラグランジュの平均値の定理) using DeepL. If you looks something interesting but the auto-translated English is not good enough to understand it, feel free to let me know at [@nishio_en](https://twitter.com/nishio_en). I'm very happy to spread my thought to non-Japanese readers.