---
title: "Lower fixed binomial coefficient → negative binomial theorem"
---

$\binom{A+i}{A} = [x^i] \sum_n \binom{A+n}{A}x^n = [x^i]\frac{1}{(1-x)^{A+1}} $

- [[negative binomial theorem]]
- $(1-x)^{-d} = \sum_{n=0}^\infty \binom{n+d-1}{d-1}x^n$


- [[binomial coefficient of under-fixation]] → [[negative binomial theorem]]

facing the opposite direction
- [[Power series → binomial coefficient]] :
- $[x^B]\frac{1}{(1-x)^{A}} = \binom{A+B-1}{A-1}$


relevance
- [Infinite sums with respect to the first argument of the binomial coefficients (mother function) - Skol's Wisdom Book](https://scol.hatenablog.com/entry/2019/06/02/190000)
    - This is [[generating function]].

---
This page is auto-translated from [/nishio/下固定の二項係数→負の二項定理](https://scrapbox.io/nishio/下固定の二項係数→負の二項定理) using DeepL. If you looks something interesting but the auto-translated English is not good enough to understand it, feel free to let me know at [@nishio_en](https://twitter.com/nishio_en). I'm very happy to spread my thought to non-Japanese readers.