---
title: "Negative binomial theorem and redundant combinations"
---

- $(1-x)^{-d} = \sum_{n=0}^\infty H_{d-1}^{n+1} x^n$

- [[negative binomial theorem]] :
- $(1-x)^{-d} = \sum_{n=0}^\infty \binom{n+d-1}{d-1}x^n$
- [[nested combination]] :
- $H^n_k = \binom{n + k - 1}{k} = \frac{(n + k - 1)!}{k!(n - 1)!}$

---
This page is auto-translated from [/nishio/負の二項定理と重複組合せ](https://scrapbox.io/nishio/負の二項定理と重複組合せ) using DeepL. If you looks something interesting but the auto-translated English is not good enough to understand it, feel free to let me know at [@nishio_en](https://twitter.com/nishio_en). I'm very happy to spread my thought to non-Japanese readers.